Enable more tests

test/Rust7.fst
@@ -7,77 +7,79 @@ open LowStar.BufferOps
 open FStar
 open FStar.HyperStack.ST
 
-// val add_carry_u32:
-//   x:U32.t
-//   -> y:U32.t
-//   -> r:B.lbuffer U32.t 1
-//   -> p:B.lbuffer U32.t 1 ->
-//   Stack U32.t
-//   (requires fun h -> B.live h r /\ B.live h p)
-//   (ensures  fun h0 c h1 -> True)
-//     // modifies1 r h0 h1 /\ v c <= 1 /\
-//     // (let r = Seq.index (as_seq h1 r) 0 in
-//     // v r + v c * pow2 (bits t) == v x + v y + v cin))
+val add_carry_u32:
+  x:U32.t
+  -> y:U32.t
+  -> r:B.lbuffer U32.t 1
+  -> p:B.lbuffer U32.t 1 ->
+  Stack U32.t
+  (requires fun h -> B.live h r /\ B.live h p)
+  (ensures  fun h0 c h1 -> True)
+    // modifies1 r h0 h1 /\ v c <= 1 /\
+    // (let r = Seq.index (as_seq h1 r) 0 in
+    // v r + v c * pow2 (bits t) == v x + v y + v cin))
 
-// let add_carry_u32 x y r p =
-//   let z = B.index p 0ul in
-//   let res = U32.add_mod x y in
-//   let res = U32.add_mod res z in
-//   // let c = (U32.shift_right res 32ul) in
-//   B.upd r 0ul res;
-//   0ul
+let add_carry_u32 x y r p =
+  let z = B.index p 0ul in
+  let res = U32.add_mod x y in
+  let res = U32.add_mod res z in
+  // let c = (U32.shift_right res 32ul) in
+  B.upd r 0ul res;
+  0ul
 
-// let test_alloca (x: UInt32.t)  : Stack UInt32.t
-//   (requires (fun h0 -> True))
-//   (ensures (fun h0 r h1 -> True)) =
-//   push_frame();
-//   let ptr = B.alloca 0ul 10ul in
-//   B.upd ptr 0ul x;
-//   let res = B.index ptr 0ul in
-//   pop_frame();
-//   x
+let test_alloca (x: UInt32.t)  : Stack UInt32.t
+  (requires (fun h0 -> True))
+  (ensures (fun h0 r h1 -> True)) =
+  push_frame();
+  let ptr = B.alloca 0ul 10ul in
+  B.upd ptr 0ul x;
+  let res = B.index ptr 0ul in
+  pop_frame();
+  x
 
-// // simple for loop example - note that there is no framing
-// let loop (ptr:B.lbuffer U32.t 10)  : Stack UInt32.t
-//   (requires (fun h0 -> B.live h0 ptr))
-//   (ensures (fun h0 r h1 -> True)) =
-//   push_frame();
-//   C.Loops.for 0ul 0ul
-//     (fun h i -> B.live h ptr)
-//     (fun i -> B.upd ptr i 1ul);
-//   C.Loops.for 0ul 1ul
-//     (fun h i -> B.live h ptr)
-//     (fun i -> B.upd ptr i 1ul);
-//   C.Loops.for 0ul 10ul
-//     (fun h i -> B.live h ptr)
-//     (fun i -> B.upd ptr i 1ul);
-//   let sum = B.index ptr 0ul in
-//   pop_frame();
-//   sum
+// simple for loop example - note that there is no framing
+let loop (ptr:B.lbuffer U32.t 10)  : Stack UInt32.t
+  (requires (fun h0 -> B.live h0 ptr))
+  (ensures (fun h0 r h1 -> True)) =
+  push_frame();
+  C.Loops.for 0ul 0ul
+    (fun h i -> B.live h ptr)
+    (fun i -> B.upd ptr i 1ul);
+  C.Loops.for 0ul 1ul
+    (fun h i -> B.live h ptr)
+    (fun i -> B.upd ptr i 1ul);
+  C.Loops.for 0ul 10ul
+    (fun h i -> B.live h ptr)
+    (fun i -> B.upd ptr i 1ul);
+  let sum = B.index ptr 0ul in
+  pop_frame();
+  sum
 
 
-// let loop_alloc ()  : Stack UInt32.t
-//   (requires (fun h0 -> True))
-//   (ensures (fun h0 r h1 -> True)) =
-//   push_frame();
-//   let ptr = B.alloca 0ul 10ul in
-//   C.Loops.for 0ul 9ul
-//     (fun h i -> B.live h ptr)
-//     (fun i -> B.upd ptr i 1ul);
-//   let sum = B.index ptr 0ul in
-//   pop_frame();
-//   sum
+let loop_alloc ()  : Stack UInt32.t
+  (requires (fun h0 -> True))
+  (ensures (fun h0 r h1 -> True)) =
+  push_frame();
+  let ptr = B.alloca 0ul 10ul in
+  C.Loops.for 0ul 9ul
+    (fun h i -> B.live h ptr)
+    (fun i -> B.upd ptr i 1ul);
+  let sum = B.index ptr 0ul in
+  pop_frame();
+  sum
 
 let root_alias (): Stack unit (fun _ -> True) (fun _ _ _ -> True) =
   push_frame ();
   let x = B.alloca 0UL 6ul in
   let x0 = B.sub x 0ul 2ul in
-  // let x1 = B.sub x 2ul 2ul in
+  let x1 = B.sub x 2ul 2ul in
 
-  // let x00 = B.sub x0 0ul 1ul in
-  // let x01 = B.sub x0 1ul 1ul in
+  let x00 = B.sub x0 0ul 1ul in
+  let x01 = B.sub x0 1ul 1ul in
 
-  // B.upd x00 0ul 2UL;
-  B.upd x0 0ul 2UL;
-  // B.upd x 0ul 4UL;
+  B.upd x00 0ul 2UL;
+  (* B.upd x0 0ul 2UL; *)
+  (* B.upd x 0ul 4UL; *)
   pop_frame()
+
+let main_ () = 0l
